store case done

theories/ftlr/Store.v
@@ -1,57 +1,38 @@
 From iris.proofmode Require Import tactics.
 From iris.program_logic Require Import weakestpre adequacy lifting.
 From stdpp Require Import base.
-From cap_machine Require Export logrel monotone.
+From cap_machine Require Export logrel.
 From cap_machine Require Import ftlr_base.
 From cap_machine.rules Require Import rules_Store.
 Import uPred.
 
+
 Section fundamental.
   Context {Σ:gFunctors} {memg:memG Σ} {regg:regG Σ}
-          {stsg : STSG Addr region_type Σ} {heapg : heapG Σ}
-          `{MonRef: MonRefG (leibnizO _) CapR_rtc Σ} {nainv: logrel_na_invs Σ}
+          {nainv: logrel_na_invs Σ}
           `{MachineParameters}.
 
-  Notation STS := (leibnizO (STS_states * STS_rels)).
-  Notation STS_STD := (leibnizO (STS_std_states Addr region_type)).
-  Notation WORLD := (prodO STS_STD STS). 
-  Implicit Types W : WORLD.
-
-  Notation D := (WORLD -n> (leibnizO Word) -n> iProp Σ).
-  Notation R := (WORLD -n> (leibnizO Reg) -n> iProp Σ).
+  Notation D := ((leibnizO Word) -n> iProp Σ).
+  Notation R := ((leibnizO Reg) -n> iProp Σ).
   Implicit Types w : (leibnizO Word).
   Implicit Types interp : (D).
 
-  Lemma execcPC_implies_interp W p g b e a0:
-    p = RX ∨ p = RWX ∨ p = RWLX ∧ g = Local →
-    ([∗ list] a ∈ region_addrs b e,
-     ∃ p', ⌜PermFlows p p'⌝ ∗
-       read_write_cond a p' interp
-       ∧ ⌜if pwl p
-          then region_state_pwl W a
-          else region_state_nwl W a g⌝) -∗
-      ((fixpoint interp1) W) (inr (p, g, b, e, a0)).
-  Proof.
-    iIntros (Hp) "#HR".
-    rewrite (fixpoint_interp1_eq _ (inr _)).
-    (do 2 try destruct Hp as [ | Hp]). 3:destruct Hp.
-    all:subst; auto. 
-  Qed.
 
   (* The necessary resources to close the region again, except for the points to predicate, which we will store separately *)
-  Definition region_open_resources W l ls p φ (v : Word): iProp Σ :=
-    (∃ ρ,
-        sts_state_std l ρ
-    ∗ ⌜std W !! l = Some ρ⌝
-    ∗ ⌜ρ ≠ Revoked ∧ (∀ g, ρ ≠ Static g)⌝
-    ∗ open_region_many (l :: ls) W
-    ∗ ⌜p ≠ O⌝
-    ∗ rel l p φ)%I.
+  (* Since we will store a new word into a, we do not need to remember its validity *)
+  Definition region_open_resources (a pc_a : Addr) pc_w : iProp Σ :=
+    (▷ interp pc_w ∗ ((▷ ∃ w0, a ↦ₐ w0 ∗ interp w0) ={⊤ ∖ ↑logN.@pc_a ∖ ↑logN.@a,⊤ ∖ ↑logN.@pc_a}=∗ emp))%I.
 
-  Lemma store_inr_eq {regs r p0 g0 b0 e0 a0 p1 g1 b1 e1 a1 storev}:
-    reg_allows_store regs r p0 g0 b0 e0 a0 storev →
-    read_reg_inr regs r p1 g1 b1 e1 a1 →
-    p0 = p1 ∧ g0 = g1 ∧ b0 = b1 ∧ e0 = e1 ∧ a0 = a1.
+  (* Definition region_open_resources_pc (pc_a : Addr) : iProp Σ := *)
+  (*   ((▷ ∃ w0, pc_a ↦ₐ w0 ∗ interp w0) ={⊤ ∖ ↑logN.@pc_a,⊤}=∗ emp)%I. *)
+
+  (* Definition region_open_resources_pc_read (pc_a : Addr) (P : D) pc_w : iProp Σ := *)
+  (*   (▷ P pc_w ∗ read_cond P interp ∗ ((▷ ∃ w0, pc_a ↦ₐ w0 ∗ P w0) ={⊤ ∖ ↑logN.@pc_a,⊤}=∗ emp))%I. *)
+  
+  Lemma store_inr_eq {regs r p0 b0 e0 a0 p1 b1 e1 a1}:
+    reg_allows_store regs r p0 b0 e0 a0 →
+    read_reg_inr regs r p1 b1 e1 a1 →
+    p0 = p1 ∧ b0 = b1 ∧ e0 = e1 ∧ a0 = a1.
   Proof.
       intros Hrar H3.
       pose (Hrar' := Hrar).
@@ -62,255 +43,149 @@ Section fundamental.
   Qed.
 
   (* Description of what the resources are supposed to look like after opening the region if we need to, but before closing the region up again*)
-  Definition allow_store_res W r1 r2 (regs : Reg) pc_a (pc_p : Perm) :=
-    (∃ p g b e a storev, ⌜read_reg_inr regs r1 p g b e a⌝ ∗ ⌜word_of_argument regs r2 = Some storev⌝ ∗
-    if decide (reg_allows_store regs r1 p g b e a storev ) then
-      (if decide (a ≠ pc_a) then
-         ∃ p' w, a ↦ₐ [p'] w  ∗ ⌜PermFlows p p'⌝ ∗ (region_open_resources W a [pc_a] p' interpC w)
-         else open_region pc_a W ∗ ⌜PermFlows p pc_p⌝ )
-      else open_region pc_a W)%I.
+  Definition allow_store_res r1 (regs : Reg) pc_a a p b e :=
+    (⌜read_reg_inr regs r1 p b e a⌝ ∗ 
+      if decide (reg_allows_store regs r1 p b e a ∧ a ≠ pc_a) then
+          |={⊤ ∖ ↑logN.@pc_a,⊤ ∖ ↑logN.@pc_a ∖ ↑logN.@a}=> ∃ w, a ↦ₐ w ∗ region_open_resources a pc_a w 
+    else True)%I.
 
-  Definition allow_store_mem W r1 r2 (regs : Reg) pc_a pc_p pc_w (mem : PermMem):=
-    (∃ p g b e a storev, ⌜read_reg_inr regs r1 p g b e a⌝ ∗ ⌜word_of_argument regs r2 = Some storev⌝ ∗
-    if decide (reg_allows_store regs r1 p g b e a storev) then
-      (if decide (a ≠ pc_a) then
-         ∃ p' w, ⌜mem = <[a:=(p',w)]> (<[pc_a:=(pc_p,pc_w)]> ∅)⌝ ∗
-            ⌜PermFlows p p'⌝ ∗ (region_open_resources W a [pc_a] p' interpC w)
-         else  ⌜mem = <[pc_a:=(pc_p,pc_w)]> ∅⌝ ∗ open_region pc_a W ∗ ⌜PermFlows p pc_p⌝ )
-    else  ⌜mem = <[pc_a:=(pc_p,pc_w)]> ∅⌝ ∗ open_region pc_a W)%I.
-
-  Lemma interp_hpf_eq (W : WORLD) (r : leibnizO Reg) (r1 : RegName)
-        p g b e a pc_p pc_g pc_b pc_e pc_p' w storev:
-    reg_allows_store (<[PC:=inr (pc_p, pc_g, pc_b, pc_e, a)]> r) r1 p g b e a storev
-    → PermFlows pc_p pc_p'
-    → (∀ r1 : RegName, ⌜r1 ≠ PC⌝ → ((fixpoint interp1) W) (r !r! r1))
-        -∗ read_write_cond a pc_p' interp
-        -∗ ⌜PermFlows p pc_p'⌝.
-  Proof.
-    destruct (decide (r1 = PC)).
-    - subst r1. iIntros ([? ?] ?). simplify_map_eq; auto.
-    - iIntros ((Hsomer1 & Hwa & Hwb & Hloc) Hfl) "Hreg Hinva".
-      iDestruct ("Hreg" $! r1 n) as "Hr1". simplify_map_eq. rewrite /RegLocate Hsomer1.
-      iDestruct (read_allowed_inv _ a with "Hr1") as (p'' Hfl') "#Harel'"; auto.
-      { apply andb_true_iff in Hwb as [Hle Hge].
-        split; [apply Zle_is_le_bool | apply Zlt_is_lt_bool]; auto. }
-      { by apply writeA_implies_readA in Hwa as ->. }
-      rewrite /read_write_cond.
-      iDestruct (rel_agree a p'' pc_p' with "[$Hinva $Harel']") as "[-> _]".
-      done.
-  Qed.
+  Definition allow_store_mem r1 (regs : Reg) pc_a pc_w (mem : gmap Addr Word) p b e a :=
+    (⌜read_reg_inr regs r1 p b e a⌝ ∗
+    if decide (reg_allows_store regs r1 p b e a ∧ a ≠ pc_a) then
+         ∃ w, ⌜mem = <[a:=w]> (<[pc_a:=pc_w]> ∅)⌝ ∗ region_open_resources a pc_a w
+    else ⌜mem = <[pc_a:=pc_w]> ∅⌝)%I.
+  
 
   Lemma create_store_res:
-    ∀ (W : WORLD) (r : leibnizO Reg) (p p' : Perm)
-      (g : Locality) (b e a : Addr) (r1 : RegName) (r2 : Z + RegName) (p0 : Perm)
-      (g0 : Locality) (b0 e0 a0 : Addr)(storev : Word),
-      read_reg_inr (<[PC:=inr (p, g, b, e, a)]> r) r1 p0 g0 b0 e0 a0
-      → PermFlows p p'
-      → word_of_argument (<[PC:=inr (p, g, b, e, a)]> r) r2 = Some storev
-      → (∀ r1 : RegName, ⌜r1 ≠ PC⌝ → ((fixpoint interp1) W) (r !r! r1))
-          -∗ read_write_cond a p' interp
-          -∗ open_region a W
-          -∗ sts_full_world W
-          -∗ allow_store_res W r1 r2 (<[PC:=inr (p, g, b, e, a)]> r) a p'
-          ∗ sts_full_world W.
+    ∀ (r : leibnizO Reg) (p : Perm)
+      (b e a : Addr) (r1 : RegName) (p0 : Perm)
+      (b0 e0 a0 : Addr),
+      read_reg_inr (<[PC:=inr (p, b, e, a)]> r) r1 p0 b0 e0 a0
+      → (∀ r1 : RegName, ⌜r1 ≠ PC⌝ → (fixpoint interp1) (r !r! r1))
+          -∗ allow_store_res r1 (<[PC:=inr (p, b, e, a)]> r) a a0 p0 b0 e0.
   Proof.
-    intros W r p p' g b e a r1 r2 p0 g0 b0 e0 a0 storev HVr1 Hfl Hwoa.
-    iIntros "#Hreg #Hinva Hr Hsts".
-    do 6 (iApply sep_exist_r; iExists _). iFrame "%".
+    intros r p b e a r1 p0 b0 e0 a0 HVr1.
+    iIntros "#Hreg".
+    iFrame "%".
     case_decide as Hallows.
-    -  case_decide as Haeq.
-       * destruct Hallows as (Hrinr & Hra & Hwb & HLoc).
-         apply andb_prop in Hwb as [Hle Hge].
-         rewrite /leb_addr in Hle,Hge.
-         assert (r1 ≠ PC) as n. refine (addr_ne_reg_ne Hrinr _ Haeq). by rewrite lookup_insert.
-
-         iDestruct ("Hreg" $! r1 n) as "Hvsrc".
-         rewrite lookup_insert_ne in Hrinr; last by congruence.
-         rewrite /RegLocate Hrinr.
-         iDestruct (read_allowed_inv _ a0 with "Hvsrc") as (p0' Hfl') "Hrel'".
-         { split; [apply Zle_is_le_bool | apply Zlt_is_lt_bool]; auto. }
-         { by apply writeA_implies_readA in Hra as ->. }
-         rewrite /read_write_cond.
-
-         iDestruct (region_open_prepare with "Hr") as "Hr".
-         iDestruct (readAllowed_valid_cap_implies with "Hvsrc") as %HH; eauto.
-         { by apply writeA_implies_readA. }
-         { rewrite /withinBounds /leb_addr Hle Hge. auto. }
-         destruct HH as [ρ' [Hstd' [Hnotrevoked' Hnotstatic' ] ] ].
-         (* We can finally frame off Hsts here, since it is no longer needed after opening the region*)
-         iDestruct (region_open_next _ _ _ a0 p0' ρ' with "[$Hrel' $Hr $Hsts]") as (w0) "($ & Hstate' & Hr & Ha0 & % & Hfuture & #Hval)"; eauto.
-         { intros [g1 Hcontr]. specialize (Hnotstatic' g1); contradiction. }
-         { apply not_elem_of_cons. split; auto. apply not_elem_of_nil. }
-         iExists p0', w0. iSplitL "Ha0"; auto. iSplitR; auto. unfold region_open_resources.
-         iExists ρ'. iFrame "%". iFrame. by iFrame "#".
-      * subst a0. iFrame. iApply interp_hpf_eq; eauto.
-    - iFrame.
+    - destruct Hallows as ((Hrinr & Hra & Hwb) & Haeq).
+      apply andb_prop in Hwb as [Hle Hge].
+      revert Hle Hge. rewrite !/leb_addr !Z.leb_le Z.ltb_lt =>Hle Hge.
+      assert (r1 ≠ PC) as n. refine (addr_ne_reg_ne Hrinr _ Haeq). by rewrite lookup_insert.
+      iDestruct ("Hreg" $! r1 n) as "Hvsrc".
+      rewrite lookup_insert_ne in Hrinr; last by congruence.
+      rewrite /RegLocate Hrinr.
+      iAssert (inv (logN.@a0) ((interp_ref_inv a0) interp))%I as "#Hinva".
+      { iApply (write_allowed_inv with "Hvsrc"); auto. }
+      iFrame "∗ #". 
+      iMod (inv_open with "Hinva") as "[Hinv Hcls']";[solve_ndisj|]. 
+      iDestruct "Hinv" as (w) "[>Ha0 #Hinv]". 
+      iExists w. iFrame. done.
+    - done.  
   Qed.
+
 
   Lemma store_res_implies_mem_map:
-    ∀ (W : WORLD) (r : leibnizO Reg) (p' : Perm)
-       (a : Addr) (w : Word) (r1 : RegName) (r2 : Z + RegName),
-      allow_store_res W r1 r2 r a p'
-      -∗ a ↦ₐ[p'] w
-      -∗ ∃ mem0 : PermMem,
-          allow_store_mem W r1 r2 r a p' w mem0
-            ∗ ▷ ([∗ map] a0↦pw ∈ mem0, ∃ (p0 : Perm) (w0 : leibnizO Word),
-                ⌜pw = (p0, w0)⌝ ∗ a0 ↦ₐ[p0] w0).
+    ∀ (r : leibnizO Reg)
+       (a a0 : Addr) (w : Word) (r1 : RegName) p1 b1 e1,
+      allow_store_res r1 r a a0 p1 b1 e1
+      -∗ a ↦ₐ w
+      ={⊤ ∖ ↑logN.@a, if decide (reg_allows_store r r1 p1 b1 e1 a0 ∧ a0 ≠ a) then ⊤ ∖ ↑logN.@a ∖ ↑logN.@a0
+                      else ⊤ ∖ ↑logN.@a}=∗ ∃ mem0 : gmap Addr Word,
+          allow_store_mem r1 r a w mem0 p1 b1 e1 a0
+            ∗ ▷ ([∗ map] a0↦w ∈ mem0, a0 ↦ₐ w).
   Proof.
-    intros W r p' a w r1 r2.
+    intros r a a0 w r1 p1 b1 e1.
     iIntros "HStoreRes Ha".
-    iDestruct "HStoreRes" as (p1 g1 b1 e1 a1 storev) "(% & % & HStoreRes)".
+    iDestruct "HStoreRes" as "(% & HStoreRes)".
 
     case_decide as Hallows.
-    - case_decide as Haeq.
-      ++ pose(Hallows' := Hallows). destruct Hallows as (Hrinr & Hra & Hwb & HLoc).
-         iDestruct "HStoreRes" as (p'0 w0) "[HStoreCh HStoreRest]".
-         iExists _.
-         iSplitL "HStoreRest".
-        + iExists p1,g1,b1,e1,a1,storev. iFrame "%".
-          case_decide; last by exfalso. case_decide; last by exfalso.
-          iExists p'0,w0. iSplitR; auto.
-        + iNext.
-          iApply memMap_resource_2ne; auto; iFrame.
-      ++ iExists _.
-         iSplitL "HStoreRes".
-        + iExists p1,g1,b1,e1,a1,storev. iFrame "%".
-          case_decide; last by exfalso. case_decide; first by exfalso.
-          iFrame. auto.
-        + iNext. by iApply memMap_resource_1.
+    - iMod "HStoreRes" as (w0) "[Ha0 HStoreRest]". 
+      iExists _. 
+      iSplitL "HStoreRest".
+      * iFrame "%". 
+        case_decide; last by exfalso.        
+        iExists w0. iSplitR; auto.
+      * iModIntro. iNext.
+        destruct Hallows as ((Hrinr & Hra & Hwb) & Hne).
+        iApply memMap_resource_2ne; auto; iFrame. 
     - iExists _.
-      iSplitL "HStoreRes".
-      + iExists p1,g1,b1,e1,a1,storev. iFrame "%".
-        case_decide; first by exfalso. iFrame. auto.
-      + iNext. by iApply memMap_resource_1.
-    Qed.
+      iSplitR "Ha". 
+      + iFrame "%".
+        case_decide; first by exfalso. auto.
+      + iModIntro. iNext. by iApply memMap_resource_1.
+  Qed.
 
+  
   Lemma mem_map_implies_pure_conds:
-    ∀ (W : WORLD) (r : leibnizO Reg) (p p' : Perm)
-      (g : Locality) (b e a : Addr) (w : Word) (r1 : RegName) (r2 : Z + RegName)
-      (mem0 : PermMem),
-        p' ≠ O →
-        allow_store_mem W r1 r2 r a p' w mem0
-        -∗ ⌜mem0 !! a = Some (p', w)⌝
-          ∗ ⌜allow_store_map_or_true r1 r2 r mem0⌝.
+    ∀ (r : leibnizO Reg) 
+      (a a0 : Addr) (w : Word) (r1 : RegName)
+      (mem0 : gmap Addr Word) p b e,
+        allow_store_mem r1 r a w mem0 p b e a0
+        -∗ ⌜mem0 !! a = Some w⌝
+          ∗ ⌜allow_store_map_or_true r1 r mem0⌝.
   Proof.
-    iIntros (W r p p' g b e a w r1 r2 mem0 Hp'O) "HStoreMem".
-    iDestruct "HStoreMem" as (p1 g1 b1 e1 a1 storev) "(% & % & HStoreRes)".
+    iIntros (r a a0 w r1 mem0 p b e) "HStoreMem".
+    iDestruct "HStoreMem" as "(% & HStoreRes)".
     case_decide as Hallows.
-    - case_decide as Haeq.
-      + pose(Hallows' := Hallows). destruct Hallows' as (Hrinr & Hra & Hwb & HLoc).
-        (* case_decide as Haeq. *)
-        iDestruct "HStoreRes" as (p'0 w0 ->) "[% _]".
-        iSplitR. rewrite lookup_insert_ne; auto. by rewrite lookup_insert.
-        iExists p1,g1,b1,e1,a1,storev.
-        iPureIntro. repeat split; auto.
-        case_decide; last by exfalso.
-        exists p'0,w0. by simplify_map_eq.
-      + subst a. iDestruct "HStoreRes" as "[-> [HStoreRes % ] ]".
-         iSplitR. by rewrite lookup_insert.
-         iExists p1,g1,b1,e1,a1,storev. repeat iSplitR; auto.
-         case_decide as Hdec1; last by done.
-         iExists p',w.  by rewrite lookup_insert.
-    - iDestruct "HStoreRes" as "[-> HStoreRes ]".
+    - pose(Hallows' := Hallows).
+      destruct Hallows' as ((Hrinr & Hra & Hwb) & Hne).
+      iDestruct "HStoreRes" as (w0 ->) "HStoreRest".
+      iSplitR. rewrite lookup_insert_ne; auto. by rewrite lookup_insert.
+      iExists p,b,e,a0. iSplit;auto. 
+      iPureIntro. case_decide;auto.
+      exists w0. by simplify_map_eq.
+    - iDestruct "HStoreRes" as "->".
       iSplitR. by rewrite lookup_insert.
-      iExists p1,g1,b1,e1,a1,storev. repeat iSplitR; auto.
-      case_decide as Hdec1; last by done. by exfalso.
+      iExists p,b,e,a0. repeat iSplitR; auto.
+      case_decide as Hdec1; last by done.
+      apply not_and_l in Hallows as [Hallows | Hallows]; try contradiction.
+      assert (a0 = a) as ->.
+      { apply z_of_eq, Z.eq_dne. intros Hcontr. apply Hallows. by intros ->. } 
+      simplify_map_eq. eauto. 
   Qed.
 
-  Lemma storev_interp_mono W (r : Reg) (r1 : RegName) (r2 : Z + RegName) p g b e a p' ρ storev:
-     PermFlows p p'
-     → word_of_argument r r2 = Some storev
-     → reg_allows_store r r1 p g b e a storev
-     → std W !! a = Some ρ
-     → ((fixpoint interp1) W) (inr (p,g,b,e,a))
-       -∗ monotonicity_guarantees_region ρ storev p' interpC.
-   Proof.
-     iIntros (Hpf Hwoa Hras Hststd) "HInt".
-     destruct Hras as (Hrir & Hwa & Hwb & Hloc).
-     destruct storev as [z | cap].
-     - iApply (interp_monotone_generalZ with "[HInt]" ); eauto.
-     - destruct r2. cbn in Hwoa; inversion Hwoa; by exfalso.
-       destruct_cap cap. cbn in Hwoa.
-       destruct (r !! r0); inversion Hwoa; clear Hwoa; subst w.
-       iApply (interp_monotone_generalW with "[HInt]" ); eauto.
-       apply orb_true_iff. destruct Hloc.
-       *  cbn in H. left. by apply negb_true_iff.
-       *  right. naive_solver.
-  Qed.
-
-  (* Note that we turn in all information that we might have on the monotonicity of the current PC value, so that in the proof of the ftlr case itself, we do not have to worry about whether the PC was written to or not when we close the last location pc_a in the region *)
    Lemma mem_map_recover_res:
-    ∀ (W : WORLD) (r : Reg) (p' : Perm)
-       (pc_w : Word) (r1 : RegName) (r2 : Z + RegName) (p0 p'0 pc_p pc_p' : Perm)
-       (g0 pc_g : Locality) (b0 e0 a0 pc_b pc_e pc_a : Addr) (mem0 : PermMem) (oldv storev : Word) (ρ : region_type),
-      word_of_argument (<[PC:=inr (pc_p, pc_g, pc_b, pc_e, pc_a)]> r) r2 = Some storev
-      → reg_allows_store (<[PC:=inr (pc_p, pc_g, pc_b, pc_e, pc_a)]> r) r1 p0 g0 b0 e0 a0 storev
-      → std W !! pc_a = Some ρ
-      → mem0 !! a0 = Some (p'0, oldv) (*?*)
-      → allow_store_mem W r1 r2 (<[PC:=inr (pc_p, pc_g, pc_b, pc_e, pc_a)]> r) pc_a pc_p' pc_w mem0
-        -∗ (∀ r1 : RegName, ⌜r1 ≠ PC⌝ → ((fixpoint interp1) W) (r !r! r1))
-        -∗ ((fixpoint interp1) W) (inr(pc_p, pc_g, pc_b, pc_e, pc_a))
-        -∗ ((fixpoint interp1) W) pc_w
-        -∗ monotonicity_guarantees_region ρ pc_w pc_p' interpC
-        -∗ ([∗ map] a0↦pw ∈ <[a0 := (p'0, storev)]> mem0, ∃ (p0 : Perm) (w0 : Word),
-                ⌜pw = (p0, w0)⌝ ∗ a0 ↦ₐ[p0] w0)
-        -∗ ∃ v, open_region pc_a W ∗ pc_a ↦ₐ[pc_p'] v ∗ ((fixpoint interp1) W) v ∗ monotonicity_guarantees_region ρ v pc_p' interpC.
-   Proof.
-    intros W r p' pc_w r1 r2 p0 p'0 pc_p pc_p' g0 pc_g b0 e0 a0 pc_b pc_e pc_a mem0 oldv storev ρ Hwoa Hras Hstdst Ha0.
-    iIntros "HStoreMem #Hreg #HVPCr #Hpc_w Hpcmono Hmem".
-    iDestruct "HStoreMem" as (p1 g1 b1 e1 a1 storev1) "[% [% HStoreRes] ]".
-    destruct (store_inr_eq Hras H0) as (<- & <- &<- &<- &<-).
-    rewrite Hwoa in H1; inversion H1; simplify_eq.
-    case_decide as Hallows.
-    - iAssert (((fixpoint interp1) W) (inr (p0,g0,b0,e0,a0)))%I with "[HVPCr Hreg]" as "#HVr1".
-      { destruct Hras as [Hreg _]. destruct (decide (r1 = PC)).
-        - subst r1. rewrite lookup_insert in Hreg; by inversion Hreg.
-        - iSpecialize ("Hreg" $! r1 n). rewrite lookup_insert_ne in Hreg; last congruence. by rewrite /RegLocate Hreg.
-      }
-      iAssert (((fixpoint interp1) W) storev1)%I with "[HVPCr Hreg]" as "#HVstorev1".
-      { destruct storev1.
-        - repeat rewrite fixpoint_interp1_eq. by cbn.
-        - destruct r2. cbn in Hwoa; inversion Hwoa; by exfalso.
-          destruct_cap c. cbn in Hwoa.
-          destruct (<[PC:=inr (pc_p, pc_g, pc_b, pc_e, pc_a)]> r !! r0) eqn:Hrr0; inversion Hwoa; clear Hwoa; subst w.
-          destruct (decide (r0 = PC)).
-          + subst r0. rewrite lookup_insert in Hrr0. by inversion Hrr0.
-          + iSpecialize ("Hreg" $! r0 n).  rewrite lookup_insert_ne in Hrr0; last congruence. by rewrite /RegLocate Hrr0.
-      }
-      case_decide as Haeq.
-      + iExists pc_w.
-        destruct Hallows as [Hrinr [Hwa [Hwb Hloc] ] ].
-        iDestruct "HStoreRes" as (p'1 w') "[-> [% HLoadRes] ]".
-        rewrite lookup_insert in Ha0; inversion Ha0; clear Ha0; subst.
-        iDestruct "HLoadRes" as (ρ1) "(Hstate' & % & #Hrev & Hr & % & Hrel')".
-        iDestruct "Hrev" as %[Hnotrevoked Hnotstatic]. 
-        rewrite insert_insert memMap_resource_2ne; last auto. iDestruct "Hmem" as  "[Ha1 $]".
-        iDestruct (storev_interp_mono with "HVr1") as "Hr1Mono"; eauto.
-        iDestruct (region_close_next with "[$Hr $Ha1 $Hrel' $Hstate' $HVstorev1 $Hr1Mono]") as "Hr"; eauto.
-        { intros [g Hcontr]. specialize (Hnotstatic g); contradiction. }
-        { apply not_elem_of_cons; split; [auto|apply not_elem_of_nil]. }
-        iDestruct (region_open_prepare with "Hr") as "$". by iFrame.
-       + subst a0. iDestruct "HStoreRes" as "[-> [HStoreRes % ] ]".
-         rewrite insert_insert -memMap_resource_1.
-         rewrite lookup_insert in Ha0; inversion Ha0; simplify_eq.
-         iExists storev1. iFrame.
-         iDestruct (storev_interp_mono with "HVr1") as "Hr1Mono"; eauto.
-    - by exfalso. 
-   Qed.
-
-  Lemma store_case(W : WORLD) (r : leibnizO Reg) (p p' : Perm) (g : Locality) (b e a : Addr) (w : Word) (ρ : region_type) (dst : RegName) (src : Z + RegName) :
-    ftlr_instr W r p p' g b e a w (Store dst src) ρ.
-
+    ∀ (r : leibnizO Reg)
+       (a : Addr) (w : Word) (src : RegName) p0
+       (b0 e0 a0 : Addr) (mem0 : gmap Addr Word) storev loadv,
+      reg_allows_store r src p0 b0 e0 a0
+      → mem0 !! a0 = Some loadv
+      → allow_store_mem src r a w mem0 p0 b0 e0 a0
+        -∗ ([∗ map] a1↦w ∈ (<[a0:=storev]> mem0), a1 ↦ₐ w)
+        -∗ interp storev                
+        ={if decide (reg_allows_store r src p0 b0 e0 a0 ∧ a0 ≠ a) then ⊤ ∖ ↑logN.@a ∖ ↑logN.@a0 else ⊤ ∖ ↑logN.@a,⊤ ∖ ↑logN.@a}=∗
+            if decide (reg_allows_store r src p0 b0 e0 a0 ∧ a0 = a) then a ↦ₐ storev else a ↦ₐ w. 
   Proof.
-    intros Hp Hsome i Hbae Hfp Hpwl Hregion [Hnotrevoked Hnotstatic] HO Hi.
-    iIntros "#IH #Hinv #Hreg #Hinva Hmono #Hw Hsts Hown".
-    iIntros "Hr Hstate Ha HPC Hmap".
+    intros r a w src p0 b0 e0 a0 mem0 storev loadv Hrar Hloadv.
+    iIntros "HLoadMem Hmem Hvalid".
+    iDestruct "HLoadMem" as "[% HLoadRes]".
+    (* destruct (load_inr_eq Hrar H0) as (<- & <- &<- &<- &<-). *)
+    case_decide as Hdec. destruct Hdec as [Hallows Heq].
+    -  destruct Hallows as [Hrinr [Hra Hwb] ].
+       iDestruct "HLoadRes" as (w0) "[-> [Hval Hcls] ]".
+       simplify_map_eq. rewrite insert_insert. 
+       rewrite memMap_resource_2ne; last auto. iDestruct "Hmem" as  "[Ha1 Haw]".
+       iMod ("Hcls" with "[Ha1 Hvalid]") as "_";[iNext;iExists storev;iFrame|]. iModIntro.
+       rewrite decide_False; [done|]. apply not_and_r. right. auto. 
+    - apply not_and_r in Hdec as [| <-%dec_stable].
+      * by exfalso.
+      * iDestruct "HLoadRes" as "->".
+        rewrite insert_insert.
+        rewrite -memMap_resource_1. simplify_map_eq. by iFrame. 
+  Qed.
+
+  Lemma store_case (r : leibnizO Reg) (p : Perm) (b e a : Addr) (w : Word) (dst : RegName) (src : Z + RegName) P :
+    ftlr_instr r p b e a w (Store dst src) P.
+  Proof.
+    intros Hp Hsome i Hbae Hi.
+    iIntros "#IH #Hinv #Hinva #Hreg #[Hread Hwrite] Hown Ha HP Hcls HPC Hmap".
     rewrite delete_insert_delete.
     iDestruct ((big_sepM_delete _ _ PC) with "[HPC Hmap]") as "Hmap /=";
       [apply lookup_insert|rewrite delete_insert_delete;iFrame|]. simpl.
 
     (* To read out PC's name later, and needed when calling wp_load *)
-    assert(∀ x : RegName, is_Some (<[PC:=inr (p, g, b, e, a)]> r !! x)) as Hsome'.
+    assert(∀ x : RegName, is_Some (<[PC:=inr (p, b, e, a)]> r !! x)) as Hsome'.
     {
       intros. destruct (decide (x = PC)).
       rewrite e0 lookup_insert; unfold is_Some. by eexists.
@@ -318,7 +193,7 @@ Section fundamental.
     }
 
     (* Initializing the names for the values of Hsrc now, to instantiate the existentials in step 1 *)
-    assert (∃ p0 g0 b0 e0 a0 , read_reg_inr (<[PC:=inr (p, g, b, e, a)]> r) dst p0 g0 b0 e0 a0) as [p0 [g0 [b0 [e0 [a0 HVdst] ] ] ] ].
+    assert (∃ p0 b0 e0 a0 , read_reg_inr (<[PC:=inr (p, b, e, a)]> r) dst p0 b0 e0 a0) as [p0 [b0 [e0 [a0 HVdst] ] ] ].
     {
       specialize Hsome' with dst as Hdst.
       destruct Hdst as [wdst Hsomedst].
@@ -326,22 +201,21 @@ Section fundamental.
       right. by exists z. by left.
     }
 
-     assert (∃ storev, word_of_argument (<[PC:=inr (p, g, b, e, a)]> r) src = Some storev) as [storev Hwoa].
+     assert (∃ storev, word_of_argument (<[PC:=inr (p, b, e, a)]> r) src = Some storev) as [storev Hwoa].
     { destruct src; cbn.
       - by exists (inl z).
       - specialize Hsome' with r0 as Hr0.
         destruct Hr0 as [wsrc Hsomer0].
         exists wsrc. by rewrite Hsomer0.
     }
-
+    
     (* Step 1: open the region, if necessary, and store all the resources obtained from the region in allow_load_res *)
-    iDestruct (create_store_res with "Hreg Hinva Hr Hsts") as "[HStoreRes Hsts]"; eauto.
-    (* Clear helper values; they exist in the existential now *)
-    clear HVdst p0 g0 b0 e0 a0 Hwoa storev.
+    iDestruct (create_store_res with "Hreg") as "HStoreRes"; eauto.
 
+    
     (* Step2: derive the concrete map of memory we need, and any spatial predicates holding over it *)
-    iDestruct (store_res_implies_mem_map W  with "HStoreRes Ha") as (mem) "[HStoreMem HMemRes]".
-
+    iMod (store_res_implies_mem_map with "HStoreRes Ha") as (mem) "[HStoreMem >HMemRes]".
+    
     (* Step 3:  derive the non-spatial conditions over the memory map*)
     iDestruct (mem_map_implies_pure_conds with "HStoreMem") as %(HReadPC & HStoreAP); auto.
 
@@ -351,31 +225,103 @@ Section fundamental.
       apply elem_of_gmap_dom. rewrite lookup_insert_is_Some'; eauto. }
     { iSplitR "Hmap"; auto. }
     iNext. iIntros (regs' mem' retv). iDestruct 1 as (HSpec) "[Hmem Hmap]".
-
-    destruct HSpec as [* ? ? ? -> Hincr|].
+    
+    destruct HSpec as [* ? ? ? -> Hincr|* -> Hincr |* ? ? ? -> Hincr].
     { apply incrementPC_Some_inv in Hincr.
-      destruct Hincr as (?&?&?&?&?&?&?&?&?).
-      iApply wp_pure_step_later; auto. iNext.
+      destruct Hincr as (?&?&?&?&?&?&?&?).
+      iApply wp_pure_step_later; auto.
+      specialize (store_inr_eq H1 HVdst) as (-> & -> & -> & ->).
 
-      (* From this, derive value relation for the current PC*)
-      iDestruct (execcPC_implies_interp _ _ _ _ _ a  with "Hinv") as "HVPC"; eauto.
-
-      iDestruct (switch_monotonicity_formulation with "Hmono") as "Hmono"; auto.
+      (* The stored value is valid *)
+      iAssert (interp storev0) as "#Hvalidstore".
+      { destruct src; inversion H0. rewrite !fixpoint_interp1_eq. done.
+        simplify_map_eq. destruct (<[PC:=inr (x, x0, x1, x2)]> r !! r0) eqn:Hsomer0;simplify_map_eq. 
+        destruct (decide (r0 = PC)).
+        - subst. simplify_map_eq. iFrame "Hinv".
+        - simplify_map_eq. iSpecialize ("Hreg" $! _ n).
+          rewrite /RegLocate. rewrite Hsomer0. iFrame "Hreg". 
+      }
       
       (* Step 4: return all the resources we had in order to close the second location in the region, in the cases where we need to *)
-      iDestruct (mem_map_recover_res with "HStoreMem Hreg HVPC Hw Hmono Hmem") as (w') "(Hr & Ha & #HSVInterp & Hmono)"; eauto.
+      iMod (mem_map_recover_res with "HStoreMem Hmem Hvalidstore") as "Ha";[eauto|eauto|iModIntro]. 
 
-      iDestruct (switch_monotonicity_formulation with "Hmono") as "Hmono"; auto.
-
-      iDestruct (region_close with "[$Hstate $Hr $Ha $Hmono]") as "Hr"; eauto.
-      { destruct ρ;auto;[..|specialize (Hnotstatic g1)];contradiction. }
+      iMod ("Hcls" with "[HP Ha]").
+      { simplify_map_eq.
+        case_decide as Hwrite. 
+        - case_decide.
+          + iNext. iExists storev.
+            iDestruct ("Hwrite" with "Hvalidstore") as "HPstore".
+            iFrame "∗ #". 
+          + iNext. iExists w. iFrame.
+        - rewrite decide_False. iNext. iExists w. iFrame.
+          intros [Hcontr ->].
+          apply Hwrite. exists dst.
+          rewrite /RegLocate. 
+          destruct Hcontr as (Hlookup & Hwa & Hwb). simplify_map_eq.
+          apply andb_prop in Hwb. 
+          revert Hwb. rewrite Z.leb_le Z.ltb_lt. auto.
+      }
+      
       simplify_map_eq.
-
-      iApply ("IH" with "[%] [] [Hmap] [$Hr] [$Hsts] [$Hown]"); auto.
-      { cbn. auto. }
-      { rewrite insert_insert. iApply "Hmap". }
+      rewrite insert_insert.
+      
+      iApply ("IH" with "[%] [] Hmap [$Hown]");auto.
+      { rewrite !fixpoint_interp1_eq /=. destruct Hp as [-> | ->]; by iFrame "#". }
     }
-    { iApply wp_pure_step_later; auto. iNext. iApply wp_value; auto. iIntros; discriminate. }
+    { rewrite /allow_store_res /allow_store_mem.
+      destruct (decide (reg_allows_store (<[PC:=inr (p, b, e, a)]> r) dst p0 b0 e0 a0 ∧ a0 ≠ a)).
+      - iDestruct "HStoreMem" as "(%&H)".
+        iDestruct "H" as (w') "(->&[Hres Hcls'])". rewrite /region_open_resources.
+        destruct a1. simplify_map_eq. rewrite memMap_resource_2ne; last auto.
+        iDestruct "Hmem" as "[Ha0 Ha]". 
+        iMod ("Hcls'" with "[Ha0 Hres]");[iExists w';iFrame|iModIntro].
+        iMod ("Hcls" with "[Ha HP]");[iExists w;iFrame|iModIntro]. 
+        iApply wp_pure_step_later; auto.
+        iApply wp_value; auto. iNext. iIntros; discriminate.
+      - iModIntro. iDestruct "HStoreMem" as "(_&->)". rewrite -memMap_resource_1. 
+        iMod ("Hcls" with "[Hmem HP]");[iExists w;iFrame|iModIntro]. 
+        iApply wp_pure_step_later; auto.
+        iApply wp_value; auto. iNext. iIntros; discriminate.
+    }
+    { (* The stored value is valid *)
+      iAssert (interp storev0) as "#Hvalidstore".
+      { destruct src; inversion H0. rewrite !fixpoint_interp1_eq. done.
+        simplify_map_eq. destruct (<[PC:=inr (p,b,e,a)]> r !! r0) eqn:Hsomer0;simplify_map_eq. 
+        destruct (decide (r0 = PC)).
+        - subst. simplify_map_eq. iFrame "Hinv".
+        - simplify_map_eq. iSpecialize ("Hreg" $! _ n).
+          rewrite /RegLocate. rewrite Hsomer0. iFrame "Hreg". 
+      }
+
+      iDestruct "HStoreMem" as "(%&H)".
+      specialize (store_inr_eq H1 HVdst) as (-> & -> & -> & ->).
+      destruct (decide (reg_allows_store (<[PC:=inr (p, b, e, a)]> r) dst p0 b0 e0 a0 ∧ a0 ≠ a)).
+      - destruct a1. simplify_map_eq.
+        iDestruct "H" as (w') "(->&[Hres Hcls'])". rewrite /region_open_resources.
+        rewrite insert_insert. 
+        rewrite memMap_resource_2ne; last auto.
+        iDestruct "Hmem" as "[Ha0 Ha]".
+        iMod ("Hcls'" with "[Ha0 Hres]");[iExists storev;iFrame "∗ #"|iModIntro].
+        iMod ("Hcls" with "[Ha HP]");[iExists w;iFrame|iModIntro].
+        iApply wp_pure_step_later; auto.
+        iApply wp_value; auto. iNext. iIntros; discriminate.
+      - apply not_and_r in n. destruct n;[contradiction|].
+        assert (a0 = a) as ->.
+        { revert H4; clear; intros. apply z_of_eq. apply Z.eq_dne. intros Hcontr.
+          apply H4. intros z_of_neq. solve_addr. }
+        case_decide. 
+        + iDestruct "H" as "->".
+          rewrite insert_insert -memMap_resource_1.
+          iModIntro.
+          iMod ("Hcls" with "[Hmem]").
+          { iNext. iExists storev0. iFrame. iApply "Hwrite". iFrame "Hvalidstore". }
+          iModIntro. iApply wp_pure_step_later; auto.
+          iApply wp_value; auto. iNext. iIntros; discriminate.
+        + simplify_map_eq. exfalso. apply H5. exists dst. 
+          rewrite /RegLocate. destruct H1 as (Hlookup & Hwa & Hwb).
+          apply andb_prop in Hwb. revert Hwb; rewrite Z.leb_le Z.ltb_lt =>Hwb.
+          rewrite Hlookup. destruct Hwb. repeat split;auto. 
+    }
     Unshelve. all: auto.
   Qed.
 
