theories/ftlr/ftlr_base.v
@@ -31,7 +31,8 @@ Section fundamental.
     -∗ (fixpoint interp1) (inr (p, b, e, a)) 
     -∗ inv (logN.@a) (∃ w0 : leibnizO Word, a ↦ₐ w0 ∗ P w0)
     -∗ (∀ r1 : RegName, ⌜r1 ≠ PC⌝ → (fixpoint interp1) (r !r! r1))
-    -∗ ▷ □ (∀ w0 : Word, P w0 -∗ (fixpoint interp1) w0)
+    -∗ ▷ □ (∀ w : Word, P w -∗ (fixpoint interp1) w)
+            ∗ (if decide (writeAllowed_in_r_a (<[PC:=inr (p, b, e, a)]> r) a) then ▷ □ (∀ w : Word, (fixpoint interp1) w -∗ P w) else emp)
     -∗ na_own logrel_nais ⊤
     -∗ a ↦ₐ w
     -∗ ▷ P w
@@ -43,6 +44,7 @@ Section fundamental.
         @ ⊤ ∖ ↑logN.@a {{ v, |={⊤ ∖ ↑logN.@a,⊤}=> WP Seq (of_val v)
                                                     {{ v0, ⌜v0 = HaltedV⌝
                                                            → ∃ r1 : Reg, full_map r1 ∧ registers_mapsto r1
-                                                             ∗ na_own logrel_nais ⊤ }} }}. 
+                                                                                                        ∗ na_own logrel_nais ⊤ }} }}.
+
 
 End fundamental.
