theories/fundamental.v
@@ -1,4 +1,4 @@
-From cap_machine.ftlr Require Export Jmp Jnz Mov Load. (* Jnz Get AddSubLt IsPtr Lea Load Mov Store Restrict Subseg LoadU StoreU PromoteU *)
+From cap_machine.ftlr Require Export Jmp Jnz Mov Load Store. (* Jnz Get AddSubLt IsPtr Lea Load Mov Store Restrict Subseg LoadU StoreU PromoteU *)
 From iris.proofmode Require Import tactics.
 From iris.program_logic Require Import weakestpre adequacy lifting.
 From stdpp Require Import base.
@@ -57,7 +57,7 @@ Section fundamental.
       assert ((b <= a)%a ∧ (a < e)%a) as Hbae.
       { eapply in_range_is_correctPC; eauto.
         unfold le_addr; omega. }
-      iDestruct (read_allowed_inv with "Hinv") as (P) "(Hinva & Hread)";[eauto|destruct Hp as [-> | ->];auto|].
+      iDestruct (read_allowed_inv_regs with "[] Hinv") as (P) "(#Hinva & #Hread)";[eauto|destruct Hp as [-> | ->];auto|iFrame "% #"|].
       rewrite /interp_ref_inv /=. 
       iInv (logN.@a) as (w) "[>Ha HP]" "Hcls". 
       iDestruct ((big_sepM_delete _ _ PC) with "Hmreg") as "[HPC Hmap]"; 
@@ -76,7 +76,7 @@ Section fundamental.
         iApply (load_case with "[] [] [] [] [] [Hown] [Ha] [HP] [Hcls] [HPC] [Hmap]");
           try iAssumption; eauto.
       + (* Store *)
-        iApply (store_case with "[] [] [] [] [Hmono] [] [Hsts] [Hown] [Hr] [Hstate] [Ha] [HPC] [Hmap]");
+        iApply (store_case with "[] [] [] [] [] [Hown] [Ha] [HP] [Hcls] [HPC] [Hmap]");
           try iAssumption; eauto.
       + (* Lt *)
         iApply (add_sub_lt_case with "[] [] [] [] [Hmono] [] [Hsts] [Hown] [Hr] [Hstate] [Ha] [HPC] [Hmap]");
